# Lesson 7: Completing the Square - Practice Worksheet

## Part A: Basic Completing the Square

1. Complete the square for each of the following expressions:
   a) $x^2 + 6x$
   b) $x^2 - 8x$
   c) $x^2 + 5x$
   d) $x^2 - 3x$

2. Complete the square for each of the following expressions and simplify:
   a) $x^2 + 10x + 7$
   b) $x^2 - 12x + 20$
   c) $x^2 + 7x - 15$
   d) $x^2 - 5x - 24$

3. Rewrite each quadratic expression in the form $a(x - h)^2 + k$:
   a) $2x^2 + 12x + 10$
   b) $3x^2 - 18x + 15$
   c) $-4x^2 + 24x - 20$
   d) $5x^2 + 30x + 50$

## Part B: Finding the Vertex Form

4. Convert each quadratic function to vertex form $f(x) = a(x - h)^2 + k$ by completing the square:
   a) $f(x) = x^2 + 8x + 12$
   b) $f(x) = x^2 - 6x + 5$
   c) $f(x) = 2x^2 + 16x + 35$
   d) $f(x) = -3x^2 + 12x - 8$

5. For each function in question 4, identify:
   a) The vertex $(h, k)$
   b) The axis of symmetry
   c) Whether the parabola opens upward or downward
   d) The minimum or maximum value of the function

6. Convert each quadratic function to vertex form and identify the vertex:
   a) $f(x) = x^2 + x - 6$
   b) $f(x) = 2x^2 - 4x + 5$
   c) $f(x) = -x^2 + 6x - 8$
   d) $f(x) = 3x^2 + 3x - 2$

## Part C: Solving Quadratic Equations by Completing the Square

7. Solve each equation by completing the square:
   a) $x^2 + 6x + 8 = 0$
   b) $x^2 - 10x + 24 = 0$
   c) $x^2 + 5x - 14 = 0$
   d) $x^2 - 7x - 18 = 0$

8. Solve each equation by completing the square:
   a) $2x^2 + 12x + 10 = 0$
   b) $3x^2 - 6x - 24 = 0$
   c) $-4x^2 + 8x + 12 = 0$
   d) $5x^2 + 20x + 15 = 0$

9. Solve each equation by completing the square:
   a) $x^2 + 4x = 12$
   b) $x^2 - 6x = -5$
   c) $2x^2 + 8x = 16$
   d) $3x^2 - 12x = -9$

## Part D: Applications

10. A rectangular garden has a length that is 3 meters more than its width. If the area of the garden is 70 square meters, find its dimensions by completing the square.

11. A ball is thrown upward from a height of 2 meters with an initial velocity of 20 meters per second. The height $h$ (in meters) of the ball after $t$ seconds is given by $h(t) = -4.9t^2 + 20t + 2$.
    a) Rewrite the function in vertex form by completing the square.
    b) What is the maximum height reached by the ball?
    c) At what time does the ball reach its maximum height?
    d) When does the ball hit the ground?

12. The profit $P$ (in dollars) for a company producing $x$ items is given by $P(x) = -0.5x^2 + 100x - 1000$.
    a) Rewrite the profit function in vertex form by completing the square.
    b) How many items should be produced to maximize the profit?
    c) What is the maximum profit?
    d) What is the break-even point (where profit equals zero)?

## Part E: Challenge Problems

13. Complete the square to find the minimum value of $f(x) = 2x^2 - 8x + 13$.

14. Use completing the square to prove that the quadratic function $f(x) = ax^2 + bx + c$ (where $a \neq 0$) has its vertex at $x = -\frac{b}{2a}$.

15. A quadratic function has its vertex at $(3, -4)$ and passes through the point $(5, 0)$. Find the equation of the function in the form $f(x) = a(x - h)^2 + k$.

## Answer Key

### Part A: Basic Completing the Square

1. a) $x^2 + 6x = (x + 3)^2 - 9$
      * Half of 6 is 3, and $3^2 = 9$
   
   b) $x^2 - 8x = (x - 4)^2 - 16$
      * Half of -8 is -4, and $(-4)^2 = 16$
   
   c) $x^2 + 5x = (x + 2.5)^2 - 6.25$
      * Half of 5 is 2.5, and $(2.5)^2 = 6.25$
   
   d) $x^2 - 3x = (x - 1.5)^2 - 2.25$
      * Half of -3 is -1.5, and $(-1.5)^2 = 2.25$

2. a) $x^2 + 10x + 7 = (x + 5)^2 - 25 + 7 = (x + 5)^2 - 18$
      * Half of 10 is 5, and $5^2 = 25$
   
   b) $x^2 - 12x + 20 = (x - 6)^2 - 36 + 20 = (x - 6)^2 - 16$
      * Half of -12 is -6, and $(-6)^2 = 36$
   
   c) $x^2 + 7x - 15 = (x + 3.5)^2 - 12.25 - 15 = (x + 3.5)^2 - 27.25$
      * Half of 7 is 3.5, and $(3.5)^2 = 12.25$
   
   d) $x^2 - 5x - 24 = (x - 2.5)^2 - 6.25 - 24 = (x - 2.5)^2 - 30.25$
      * Half of -5 is -2.5, and $(-2.5)^2 = 6.25$

3. a) $2x^2 + 12x + 10 = 2(x^2 + 6x) + 10 = 2(x^2 + 6x + 9 - 9) + 10 = 2(x + 3)^2 - 18 + 10 = 2(x + 3)^2 - 8$
   
   b) $3x^2 - 18x + 15 = 3(x^2 - 6x) + 15 = 3(x^2 - 6x + 9 - 9) + 15 = 3(x - 3)^2 - 27 + 15 = 3(x - 3)^2 - 12$
   
   c) $-4x^2 + 24x - 20 = -4(x^2 - 6x) - 20 = -4(x^2 - 6x + 9 - 9) - 20 = -4(x - 3)^2 + 36 - 20 = -4(x - 3)^2 + 16$
   
   d) $5x^2 + 30x + 50 = 5(x^2 + 6x) + 50 = 5(x^2 + 6x + 9 - 9) + 50 = 5(x + 3)^2 - 45 + 50 = 5(x + 3)^2 + 5$

### Part B: Finding the Vertex Form

4. a) $f(x) = x^2 + 8x + 12$
      $= (x^2 + 8x + 16) + 12 - 16$
      $= (x + 4)^2 - 4$
      Vertex form: $f(x) = (x + 4)^2 - 4$
   
   b) $f(x) = x^2 - 6x + 5$
      $= (x^2 - 6x + 9) + 5 - 9$
      $= (x - 3)^2 - 4$
      Vertex form: $f(x) = (x - 3)^2 - 4$
   
   c) $f(x) = 2x^2 + 16x + 35$
      $= 2(x^2 + 8x) + 35$
      $= 2(x^2 + 8x + 16 - 16) + 35$
      $= 2(x + 4)^2 - 32 + 35$
      $= 2(x + 4)^2 + 3$
      Vertex form: $f(x) = 2(x + 4)^2 + 3$
   
   d) $f(x) = -3x^2 + 12x - 8$
      $= -3(x^2 - 4x) - 8$
      $= -3(x^2 - 4x + 4 - 4) - 8$
      $= -3(x - 2)^2 + 12 - 8$
      $= -3(x - 2)^2 + 4$
      Vertex form: $f(x) = -3(x - 2)^2 + 4$

5. a) For $f(x) = (x + 4)^2 - 4$:
      * Vertex: $(-4, -4)$
      * Axis of symmetry: $x = -4$
      * Opens upward (coefficient of $x^2$ is positive)
      * Minimum value: $-4$
   
   b) For $f(x) = (x - 3)^2 - 4$:
      * Vertex: $(3, -4)$
      * Axis of symmetry: $x = 3$
      * Opens upward (coefficient of $x^2$ is positive)
      * Minimum value: $-4$
   
   c) For $f(x) = 2(x + 4)^2 + 3$:
      * Vertex: $(-4, 3)$
      * Axis of symmetry: $x = -4$
      * Opens upward (coefficient of $x^2$ is positive)
      * Minimum value: $3$
   
   d) For $f(x) = -3(x - 2)^2 + 4$:
      * Vertex: $(2, 4)$
      * Axis of symmetry: $x = 2$
      * Opens downward (coefficient of $x^2$ is negative)
      * Maximum value: $4$

6. a) $f(x) = x^2 + x - 6$
      $= (x^2 + x + \frac{1}{4}) - 6 - \frac{1}{4}$
      $= (x + \frac{1}{2})^2 - \frac{25}{4}$
      Vertex: $(-\frac{1}{2}, -\frac{25}{4})$ or $(-0.5, -6.25)$
   
   b) $f(x) = 2x^2 - 4x + 5$
      $= 2(x^2 - 2x) + 5$
      $= 2(x^2 - 2x + 1 - 1) + 5$
      $= 2(x - 1)^2 - 2 + 5$
      $= 2(x - 1)^2 + 3$
      Vertex: $(1, 3)$
   
   c) $f(x) = -x^2 + 6x - 8$
      $= -(x^2 - 6x) - 8$
      $= -(x^2 - 6x + 9 - 9) - 8$
      $= -(x - 3)^2 + 9 - 8$
      $= -(x - 3)^2 + 1$
      Vertex: $(3, 1)$
   
   d) $f(x) = 3x^2 + 3x - 2$
      $= 3(x^2 + x) - 2$
      $= 3(x^2 + x + \frac{1}{4} - \frac{1}{4}) - 2$
      $= 3(x + \frac{1}{2})^2 - \frac{3}{4} - 2$
      $= 3(x + \frac{1}{2})^2 - \frac{11}{4}$
      Vertex: $(-\frac{1}{2}, -\frac{11}{4})$ or $(-0.5, -2.75)$

### Part C: Solving Quadratic Equations by Completing the Square

7. a) $x^2 + 6x + 8 = 0$
      $(x^2 + 6x + 9) + 8 - 9 = 0$
      $(x + 3)^2 - 1 = 0$
      $(x + 3)^2 = 1$
      $x + 3 = \pm 1$
      $x = -3 \pm 1$
      $x = -2$ or $x = -4$
   
   b) $x^2 - 10x + 24 = 0$
      $(x^2 - 10x + 25) + 24 - 25 = 0$
      $(x - 5)^2 - 1 = 0$
      $(x - 5)^2 = 1$
      $x - 5 = \pm 1$
      $x = 5 \pm 1$
      $x = 6$ or $x = 4$
   
   c) $x^2 + 5x - 14 = 0$
      $(x^2 + 5x + \frac{25}{4}) - 14 - \frac{25}{4} = 0$
      $(x + \frac{5}{2})^2 - \frac{81}{4} = 0$
      $(x + \frac{5}{2})^2 = \frac{81}{4}$
      $x + \frac{5}{2} = \pm \frac{9}{2}$
      $x = -\frac{5}{2} \pm \frac{9}{2}$
      $x = 2$ or $x = -7$
   
   d) $x^2 - 7x - 18 = 0$
      $(x^2 - 7x + \frac{49}{4}) - 18 - \frac{49}{4} = 0$
      $(x - \frac{7}{2})^2 - \frac{121}{4} = 0$
      $(x - \frac{7}{2})^2 = \frac{121}{4}$
      $x - \frac{7}{2} = \pm \frac{11}{2}$
      $x = \frac{7}{2} \pm \frac{11}{2}$
      $x = 9$ or $x = -2$

8. a) $2x^2 + 12x + 10 = 0$
      $2(x^2 + 6x) + 10 = 0$
      $2(x^2 + 6x + 9 - 9) + 10 = 0$
      $2(x + 3)^2 - 18 + 10 = 0$
      $2(x + 3)^2 - 8 = 0$
      $2(x + 3)^2 = 8$
      $(x + 3)^2 = 4$
      $x + 3 = \pm 2$
      $x = -3 \pm 2$
      $x = -1$ or $x = -5$
   
   b) $3x^2 - 6x - 24 = 0$
      $3(x^2 - 2x) - 24 = 0$
      $3(x^2 - 2x + 1 - 1) - 24 = 0$
      $3(x - 1)^2 - 3 - 24 = 0$
      $3(x - 1)^2 - 27 = 0$
      $3(x - 1)^2 = 27$
      $(x - 1)^2 = 9$
      $x - 1 = \pm 3$
      $x = 1 \pm 3$
      $x = 4$ or $x = -2$
   
   c) $-4x^2 + 8x + 12 = 0$
      $-4(x^2 - 2x) + 12 = 0$
      $-4(x^2 - 2x + 1 - 1) + 12 = 0$
      $-4(x - 1)^2 + 4 + 12 = 0$
      $-4(x - 1)^2 + 16 = 0$
      $-4(x - 1)^2 = -16$
      $(x - 1)^2 = 4$
      $x - 1 = \pm 2$
      $x = 1 \pm 2$
      $x = 3$ or $x = -1$
   
   d) $5x^2 + 20x + 15 = 0$
      $5(x^2 + 4x) + 15 = 0$
      $5(x^2 + 4x + 4 - 4) + 15 = 0$
      $5(x + 2)^2 - 20 + 15 = 0$
      $5(x + 2)^2 - 5 = 0$
      $5(x + 2)^2 = 5$
      $(x + 2)^2 = 1$
      $x + 2 = \pm 1$
      $x = -2 \pm 1$
      $x = -1$ or $x = -3$

9. a) $x^2 + 4x = 12$
      $x^2 + 4x + 4 = 12 + 4$
      $(x + 2)^2 = 16$
      $x + 2 = \pm 4$
      $x = -2 \pm 4$
      $x = 2$ or $x = -6$
   
   b) $x^2 - 6x = -5$
      $x^2 - 6x + 9 = -5 + 9$
      $(x - 3)^2 = 4$
      $x - 3 = \pm 2$
      $x = 3 \pm 2$
      $x = 5$ or $x = 1$
   
   c) $2x^2 + 8x = 16$
      $2(x^2 + 4x) = 16$
      $2(x^2 + 4x + 4 - 4) = 16$
      $2(x + 2)^2 - 8 = 16$
      $2(x + 2)^2 = 24$
      $(x + 2)^2 = 12$
      $x + 2 = \pm 2\sqrt{3}$
      $x = -2 \pm 2\sqrt{3}$
      $x = -2 + 2\sqrt{3}$ or $x = -2 - 2\sqrt{3}$
   
   d) $3x^2 - 12x = -9$
      $3(x^2 - 4x) = -9$
      $3(x^2 - 4x + 4 - 4) = -9$
      $3(x - 2)^2 - 12 = -9$
      $3(x - 2)^2 = 3$
      $(x - 2)^2 = 1$
      $x - 2 = \pm 1$
      $x = 2 \pm 1$
      $x = 3$ or $x = 1$

### Part D: Applications

10. Let $w$ be the width of the garden and $w + 3$ be the length.
    Area = $w(w + 3) = 70$
    $w^2 + 3w = 70$
    $w^2 + 3w - 70 = 0$
    
    Complete the square:
    $w^2 + 3w + \frac{9}{4} - \frac{9}{4} - 70 = 0$
    $(w + \frac{3}{2})^2 - \frac{9}{4} - 70 = 0$
    $(w + \frac{3}{2})^2 = \frac{9}{4} + 70 = \frac{9}{4} + \frac{280}{4} = \frac{289}{4}$
    $w + \frac{3}{2} = \pm \frac{17}{2}$
    
    Since width must be positive, $w = -\frac{3}{2} + \frac{17}{2} = 7$
    
    The dimensions of the garden are 7 meters by 10 meters.

11. a) $h(t) = -4.9t^2 + 20t + 2$
       $= -4.9(t^2 - \frac{20}{-4.9}t) + 2$
       $= -4.9(t^2 - 4.08t) + 2$
       $= -4.9(t^2 - 4.08t + 4.16 - 4.16) + 2$
       $= -4.9(t - 2.04)^2 + 20.38 + 2$
       $= -4.9(t - 2.04)^2 + 22.38$
       Vertex form: $h(t) = -4.9(t - 2.04)^2 + 22.38$
    
    b) The maximum height is 22.38 meters.
    
    c) The ball reaches its maximum height at $t = 2.04$ seconds.
    
    d) The ball hits the ground when $h(t) = 0$:
       $-4.9(t - 2.04)^2 + 22.38 = 0$
       $-4.9(t - 2.04)^2 = -22.38$
       $(t - 2.04)^2 = \frac{22.38}{4.9} \approx 4.57$
       $t - 2.04 = \pm \sqrt{4.57} \approx \pm 2.14$
       $t = 2.04 \pm 2.14$
       $t = 4.18$ or $t = -0.1$
       
       Since negative time doesn't make sense in this context, the ball hits the ground at approximately 4.18 seconds.

12. a) $P(x) = -0.5x^2 + 100x - 1000$
       $= -0.5(x^2 - 200x) - 1000$
       $= -0.5(x^2 - 200x + 10000 - 10000) - 1000$
       $= -0.5(x - 100)^2 + 5000 - 1000$
       $= -0.5(x - 100)^2 + 4000$
       Vertex form: $P(x) = -0.5(x - 100)^2 + 4000$
    
    b) The profit is maximized when $x = 100$ items.
    
    c) The maximum profit is $P(100) = 4000$ dollars.
    
    d) To find the break-even points, set $P(x) = 0$:
       $-0.5(x - 100)^2 + 4000 = 0$
       $-0.5(x - 100)^2 = -4000$
       $(x - 100)^2 = 8000$
       $x - 100 = \pm \sqrt{8000} \approx \pm 89.44$
       $x = 100 \pm 89.44$
       $x \approx 189.44$ or $x \approx 10.56$
       
       The break-even points are approximately 11 items and 189 items.

### Part E: Challenge Problems

13. $f(x) = 2x^2 - 8x + 13$
    $= 2(x^2 - 4x) + 13$
    $= 2(x^2 - 4x + 4 - 4) + 13$
    $= 2(x - 2)^2 - 8 + 13$
    $= 2(x - 2)^2 + 5$
    
    The minimum value of $f(x)$ is 5, which occurs at $x = 2$.

14. $f(x) = ax^2 + bx + c$ (where $a \neq 0$)
    $= a(x^2 + \frac{b}{a}x) + c$
    $= a(x^2 + \frac{b}{a}x + \frac{b^2}{4a^2} - \frac{b^2}{4a^2}) + c$
    $= a(x + \frac{b}{2a})^2 - \frac{b^2}{4a} + c$
    
    The vertex form is $f(x) = a(x + \frac{b}{2a})^2 + (c - \frac{b^2}{4a})$
    
    The x-coordinate of the vertex is $-\frac{b}{2a}$.

15. For a quadratic function with vertex at $(3, -4)$ and passing through $(5, 0)$:
    $f(x) = a(x - 3)^2 - 4$
    
    Since the function passes through $(5, 0)$:
    $0 = a(5 - 3)^2 - 4$
    $0 = 4a - 4$
    $4a = 4$
    $a = 1$
    
    Therefore, $f(x) = (x - 3)^2 - 4$
