# Lesson 1: Prerequisite Skills - Factoring - Practice Worksheet

## Part A: Greatest Common Factor (GCF)

1. Find the GCF of each set of terms:

- a) 12, 18
- b) 24, 36, 48
- c) 15, 45, 75
- d) 16, 24, 40

2. Factor out the GCF from each expression:

- a) 6x + 9
- b) 15y - 25
- c) 8a² + 12a
- d) 21x³ - 14x² + 7x

3. Factor out the GCF from each expression:

- a) 4x³y + 8x²y² - 12xy³
- b) 9a²b³ - 18ab⁴ + 27b⁵
- c) 5m²n³ + 15mn² - 10n
- d) 16p⁴q² - 24p³q³ + 8p²q⁴

## Part B: Factoring Trinomials with Leading Coefficient 1

4. Factor each trinomial:
   a) x² + 7x + 12
   b) x² - 8x + 15
   c) x² + 3x - 10
   d) x² - 5x - 14

5. Factor each trinomial:
   a) x² + 11x + 30
   b) x² - 13x + 42
   c) x² + 2x - 35
   d) x² - 4x - 21

6. Factor each trinomial:
   a) x² + 9x + 20
   b) x² - 11x + 28
   c) x² + 6x - 27
   d) x² - 2x - 24

## Part C: Factoring Trinomials with Leading Coefficient Other Than 1

7. Factor each trinomial:
   a) 2x² + 7x + 3
   b) 3x² - 14x + 8
   c) 4x² + 4x - 3
   d) 5x² - 13x - 6

8. Factor each trinomial:
   a) 6x² + 17x + 12
   b) 8x² - 22x + 15
   c) 9x² + 3x - 20
   d) 12x² - 11x - 15

9. Factor each trinomial:
   a) 3x² + 10x + 8
   b) 4x² - 12x + 9
   c) 6x² + 5x - 6
   d) 10x² - 29x + 10

## Part D: Special Factoring Patterns

10. Factor each difference of squares:
    a) x² - 16
    b) 25y² - 9
    c) 49a² - 64b²
    d) 121m² - 100n²

11. Factor each perfect square trinomial:
    a) x² + 6x + 9
    b) x² - 10x + 25
    c) 4y² + 12y + 9
    d) 9z² - 24z + 16

12. Factor each sum or difference of cubes:
    a) x³ + 27
    b) x³ - 8
    c) 8y³ + 1
    d) 27z³ - 125

## Part E: Mixed Factoring Problems

13. Factor each expression completely:
    a) x⁴ - 16
    b) 2x³ - 18x
    c) 3x² - 3y²
    d) 4x² + 20x + 25

14. Factor each expression completely:
    a) x³ - 4x² - 9x + 36
    b) 2x³ - 2x² - 8x + 8
    c) 6x² - 6x - 12
    d) x⁴ - 81

15. Factor each expression completely:
    a) x²y - 9y
    b) 4x² - 12xy + 9y²
    c) x³ + 3x² - 4x - 12
    d) 2x⁴ - 2x²

## Answer Key

### Part A: Greatest Common Factor (GCF)

1. a) GCF of 12 and 18 = 6
   b) GCF of 24, 36, and 48 = 12
   c) GCF of 15, 45, and 75 = 15
   d) GCF of 16, 24, and 40 = 8

2. a) 6x + 9 = 3(2x + 3)
   b) 15y - 25 = 5(3y - 5)
   c) 8a² + 12a = 4a(2a + 3)
   d) 21x³ - 14x² + 7x = 7x(3x² - 2x + 1)

3. a) 4x³y + 8x²y² - 12xy³ = 4xy(x² + 2xy - 3y²)
   b) 9a²b³ - 18ab⁴ + 27b⁵ = 9b³(a² - 2ab + 3b²)
   c) 5m²n³ + 15mn² - 10n = 5n(m²n² + 3mn - 2)
   d) 16p⁴q² - 24p³q³ + 8p²q⁴ = 8p²q²(2p² - 3pq + q²)

### Part B: Factoring Trinomials with Leading Coefficient 1

4. a) x² + 7x + 12 = (x + 3)(x + 4)
   b) x² - 8x + 15 = (x - 3)(x - 5)
   c) x² + 3x - 10 = (x + 5)(x - 2)
   d) x² - 5x - 14 = (x - 7)(x + 2)

5. a) x² + 11x + 30 = (x + 5)(x + 6)
   b) x² - 13x + 42 = (x - 6)(x - 7)
   c) x² + 2x - 35 = (x + 7)(x - 5)
   d) x² - 4x - 21 = (x - 7)(x + 3)

6. a) x² + 9x + 20 = (x + 4)(x + 5)
   b) x² - 11x + 28 = (x - 4)(x - 7)
   c) x² + 6x - 27 = (x + 9)(x - 3)
   d) x² - 2x - 24 = (x - 6)(x + 4)

### Part C: Factoring Trinomials with Leading Coefficient Other Than 1

7. a) 2x² + 7x + 3 = (2x + 1)(x + 3)
   b) 3x² - 14x + 8 = (3x - 2)(x - 4)
   c) 4x² + 4x - 3 = (2x + 3)(2x - 1)
   d) 5x² - 13x - 6 = (5x + 2)(x - 3)

8. a) 6x² + 17x + 12 = (2x + 3)(3x + 4)
   b) 8x² - 22x + 15 = (4x - 5)(2x - 3)
   c) 9x² + 3x - 20 = (3x + 4)(3x - 5)
   d) 12x² - 11x - 15 = (4x + 3)(3x - 5)

9. a) 3x² + 10x + 8 = (3x + 4)(x + 2)
   b) 4x² - 12x + 9 = (2x - 3)²
   c) 6x² + 5x - 6 = (2x + 3)(3x - 2)
   d) 10x² - 29x + 10 = (5x - 2)(2x - 5)

### Part D: Special Factoring Patterns

10. a) x² - 16 = (x + 4)(x - 4)
    b) 25y² - 9 = (5y + 3)(5y - 3)
    c) 49a² - 64b² = (7a + 8b)(7a - 8b)
    d) 121m² - 100n² = (11m + 10n)(11m - 10n)

11. a) x² + 6x + 9 = (x + 3)²
    b) x² - 10x + 25 = (x - 5)²
    c) 4y² + 12y + 9 = (2y + 3)²
    d) 9z² - 24z + 16 = (3z - 4)²

12. a) x³ + 27 = (x + 3)(x² - 3x + 9)
    b) x³ - 8 = (x - 2)(x² + 2x + 4)
    c) 8y³ + 1 = (2y + 1)(4y² - 2y + 1)
    d) 27z³ - 125 = (3z - 5)(9z² + 15z + 25)

### Part E: Mixed Factoring Problems

13. a) x⁴ - 16 = (x² + 4)(x² - 4) = (x² + 4)(x + 2)(x - 2)
    b) 2x³ - 18x = 2x(x² - 9) = 2x(x + 3)(x - 3)
    c) 3x² - 3y² = 3(x² - y²) = 3(x + y)(x - y)
    d) 4x² + 20x + 25 = (2x + 5)²

14. a) x³ - 4x² - 9x + 36 = x²(x - 4) - 9(x - 4) = (x - 4)(x² - 9) = (x - 4)(x + 3)(x - 3)
    b) 2x³ - 2x² - 8x + 8 = 2(x³ - x² - 4x + 4) = 2(x²(x - 1) - 4(x - 1)) = 2(x - 1)(x² - 4) = 2(x - 1)(x + 2)(x - 2)
    c) 6x² - 6x - 12 = 6(x² - x - 2) = 6(x + 1)(x - 2)
    d) x⁴ - 81 = (x²)² - 9² = (x² + 9)(x² - 9) = (x² + 9)(x + 3)(x - 3)

15. a) x²y - 9y = y(x² - 9) = y(x + 3)(x - 3)
    b) 4x² - 12xy + 9y² = (2x - 3y)²
    c) x³ + 3x² - 4x - 12 = x²(x + 3) - 4(x + 3) = (x + 3)(x² - 4) = (x + 3)(x + 2)(x - 2)
    d) 2x⁴ - 2x² = 2x²(x² - 1) = 2x²(x + 1)(x - 1)
