# Lesson 7: Completing the Square - Practice Worksheet

## Part A: Basic Completing the Square

1. Complete the square for each of the following expressions:
   
   ğ—®. xÂ² + 6x
   
   ğ—¯. xÂ² - 8x
   
   ğ—°. xÂ² + 5x
   
   ğ—±. xÂ² - 3x

2. Complete the square for each of the following expressions and simplify:
   
   ğ—®. xÂ² + 10x + 7
   
   ğ—¯. xÂ² - 12x + 20
   
   ğ—°. xÂ² + 7x - 15
   
   ğ—±. xÂ² - 5x - 24

3. Rewrite each quadratic expression in the form a(x - h)Â² + k:
   
   ğ—®. 2xÂ² + 12x + 10
   
   ğ—¯. 3xÂ² - 18x + 15
   
   ğ—°. -4xÂ² + 24x - 20
   
   ğ—±. 5xÂ² + 30x + 50

## Part B: Finding the Vertex Form

4. Convert each quadratic function to vertex form f(x) = a(x - h)Â² + k by completing the square:
   
   ğ—®. f(x) = xÂ² + 8x + 12
   
   ğ—¯. f(x) = xÂ² - 6x + 5
   
   ğ—°. f(x) = 2xÂ² + 16x + 35
   
   ğ—±. f(x) = -3xÂ² + 12x - 8

5. For each function in question 4, identify:
   
   ğ—®. The vertex (h, k)
   
   ğ—¯. The axis of symmetry
   
   ğ—°. Whether the parabola opens upward or downward
   
   ğ—±. The minimum or maximum value of the function

6. Convert each quadratic function to vertex form and identify the vertex:
   
   ğ—®. f(x) = xÂ² + x - 6
   
   ğ—¯. f(x) = 2xÂ² - 4x + 5
   
   ğ—°. f(x) = -xÂ² + 6x - 8
   
   ğ—±. f(x) = 3xÂ² + 3x - 2

## Part C: Solving Quadratic Equations by Completing the Square

7. Solve each equation by completing the square:
   
   ğ—®. xÂ² + 6x + 8 = 0
   
   ğ—¯. xÂ² - 10x + 24 = 0
   
   ğ—°. xÂ² + 5x - 14 = 0
   
   ğ—±. xÂ² - 7x - 18 = 0

8. Solve each equation by completing the square:
   
   ğ—®. 2xÂ² + 12x + 10 = 0
   
   ğ—¯. 3xÂ² - 6x - 24 = 0
   
   ğ—°. -4xÂ² + 8x + 12 = 0
   
   ğ—±. 5xÂ² + 20x + 15 = 0

9. Solve each equation by completing the square:
   
   ğ—®. xÂ² + 4x = 12
   
   ğ—¯. xÂ² - 6x = -5
   
   ğ—°. 2xÂ² + 8x = 16
   
   ğ—±. 3xÂ² - 12x = -9

## Part D: Applications

10. A rectangular garden has a length that is 3 meters more than its width. If the area of the garden is 70 square meters, find its dimensions by completing the square.

11. A ball is thrown upward from a height of 2 meters with an initial velocity of 20 meters per second. The height h (in meters) of the ball after t seconds is given by h(t) = -4.9tÂ² + 20t + 2.
    
    ğ—®. Rewrite the function in vertex form by completing the square.
    
    ğ—¯. What is the maximum height reached by the ball?
    
    ğ—°. At what time does the ball reach its maximum height?
    
    ğ—±. When does the ball hit the ground?

12. The profit P (in dollars) for a company producing x items is given by P(x) = -0.5xÂ² + 100x - 1000.
    
    ğ—®. Rewrite the profit function in vertex form by completing the square.
    
    ğ—¯. How many items should be produced to maximize the profit?
    
    ğ—°. What is the maximum profit?
    
    ğ—±. What is the break-even point (where profit equals zero)?

## Part E: Challenge Problems

13. Complete the square to find the minimum value of f(x) = 2xÂ² - 8x + 13.

14. Use completing the square to prove that the quadratic function f(x) = axÂ² + bx + c (where a â‰  0) has its vertex at x = -b/2a.

15. A quadratic function has its vertex at (3, -4) and passes through the point (5, 0). Find the equation of the function in the form f(x) = a(x - h)Â² + k.

## Answer Key

### Part A: Basic Completing the Square

1. a) xÂ² + 6x = (x + 3)Â² - 9
      * Half of 6 is 3, and 3Â² = 9
   
   b) xÂ² - 8x = (x - 4)Â² - 16
      * Half of -8 is -4, and (-4)Â² = 16
   
   c) xÂ² + 5x = (x + 2.5)Â² - 6.25
      * Half of 5 is 2.5, and (2.5)Â² = 6.25
   
   d) xÂ² - 3x = (x - 1.5)Â² - 2.25
      * Half of -3 is -1.5, and (-1.5)Â² = 2.25

2. a) xÂ² + 10x + 7 = (x + 5)Â² - 25 + 7 = (x + 5)Â² - 18
      * Half of 10 is 5, and 5Â² = 25
   
   b) xÂ² - 12x + 20 = (x - 6)Â² - 36 + 20 = (x - 6)Â² - 16
      * Half of -12 is -6, and (-6)Â² = 36
   
   c) xÂ² + 7x - 15 = (x + 3.5)Â² - 12.25 - 15 = (x + 3.5)Â² - 27.25
      * Half of 7 is 3.5, and (3.5)Â² = 12.25
   
   d) xÂ² - 5x - 24 = (x - 2.5)Â² - 6.25 - 24 = (x - 2.5)Â² - 30.25
      * Half of -5 is -2.5, and (-2.5)Â² = 6.25

3. a) 2xÂ² + 12x + 10 = 2(xÂ² + 6x) + 10 = 2(xÂ² + 6x + 9 - 9) + 10 = 2(x + 3)Â² - 18 + 10 = 2(x + 3)Â² - 8
   
   b) 3xÂ² - 18x + 15 = 3(xÂ² - 6x) + 15 = 3(xÂ² - 6x + 9 - 9) + 15 = 3(x - 3)Â² - 27 + 15 = 3(x - 3)Â² - 12
   
   c) -4xÂ² + 24x - 20 = -4(xÂ² - 6x) - 20 = -4(xÂ² - 6x + 9 - 9) - 20 = -4(x - 3)Â² + 36 - 20 = -4(x - 3)Â² + 16
   
   d) 5xÂ² + 30x + 50 = 5(xÂ² + 6x) + 50 = 5(xÂ² + 6x + 9 - 9) + 50 = 5(x + 3)Â² - 45 + 50 = 5(x + 3)Â² + 5

### Part B: Finding the Vertex Form

4. a) f(x) = xÂ² + 8x + 12
      = (xÂ² + 8x + 16) + 12 - 16
      = (x + 4)Â² - 4
      Vertex form: f(x) = (x + 4)Â² - 4
   
   b) f(x) = xÂ² - 6x + 5
      = (xÂ² - 6x + 9) + 5 - 9
      = (x - 3)Â² - 4
      Vertex form: f(x) = (x - 3)Â² - 4
   
   c) f(x) = 2xÂ² + 16x + 35
      = 2(xÂ² + 8x) + 35
      = 2(xÂ² + 8x + 16 - 16) + 35
      = 2(x + 4)Â² - 32 + 35
      = 2(x + 4)Â² + 3
      Vertex form: f(x) = 2(x + 4)Â² + 3
   
   d) f(x) = -3xÂ² + 12x - 8
      = -3(xÂ² - 4x) - 8
      = -3(xÂ² - 4x + 4 - 4) - 8
      = -3(x - 2)Â² + 12 - 8
      = -3(x - 2)Â² + 4
      Vertex form: f(x) = -3(x - 2)Â² + 4

5. a) For f(x) = (x + 4)Â² - 4:
      * Vertex: (-4, -4)
      * Axis of symmetry: x = -4
      * Opens upward (coefficient of xÂ² is positive)
      * Minimum value: -4
   
   b) For f(x) = (x - 3)Â² - 4:
      * Vertex: (3, -4)
      * Axis of symmetry: x = 3
      * Opens upward (coefficient of xÂ² is positive)
      * Minimum value: -4
   
   c) For f(x) = 2(x + 4)Â² + 3:
      * Vertex: (-4, 3)
      * Axis of symmetry: x = -4
      * Opens upward (coefficient of xÂ² is positive)
      * Minimum value: 3
   
   d) For f(x) = -3(x - 2)Â² + 4:
      * Vertex: (2, 4)
      * Axis of symmetry: x = 2
      * Opens downward (coefficient of xÂ² is negative)
      * Maximum value: 4

6. a) f(x) = xÂ² + x - 6
      = (xÂ² + x + 1/4) - 6 - 1/4
      = (x + 1/2)Â² - 25/4
      Vertex: (-1/2, -25/4) or (-0.5, -6.25)
   
   b) f(x) = 2xÂ² - 4x + 5
      = 2(xÂ² - 2x) + 5
      = 2(xÂ² - 2x + 1 - 1) + 5
      = 2(x - 1)Â² - 2 + 5
      = 2(x - 1)Â² + 3
      Vertex: (1, 3)
   
   c) f(x) = -xÂ² + 6x - 8
      = -(xÂ² - 6x) - 8
      = -(xÂ² - 6x + 9 - 9) - 8
      = -(x - 3)Â² + 9 - 8
      = -(x - 3)Â² + 1
      Vertex: (3, 1)
   
   d) f(x) = 3xÂ² + 3x - 2
      = 3(xÂ² + x) - 2
      = 3(xÂ² + x + 1/4 - 1/4) - 2
      = 3(x + 1/2)Â² - 3/4 - 2
      = 3(x + 1/2)Â² - 11/4
      Vertex: (-1/2, -11/4) or (-0.5, -2.75)

### Part C: Solving Quadratic Equations by Completing the Square

7. a) xÂ² + 6x + 8 = 0
      (xÂ² + 6x + 9) + 8 - 9 = 0
      (x + 3)Â² - 1 = 0
      (x + 3)Â² = 1
      x + 3 = Â±1
      x = -3 Â± 1
      x = -2 or x = -4
   
   b) xÂ² - 10x + 24 = 0
      (xÂ² - 10x + 25) + 24 - 25 = 0
      (x - 5)Â² - 1 = 0
      (x - 5)Â² = 1
      x - 5 = Â±1
      x = 5 Â± 1
      x = 6 or x = 4
   
   c) xÂ² + 5x - 14 = 0
      (xÂ² + 5x + 25/4) - 14 - 25/4 = 0
      (x + 5/2)Â² - 81/4 = 0
      (x + 5/2)Â² = 81/4
      x + 5/2 = Â±9/2
      x = -5/2 Â± 9/2
      x = 2 or x = -7
   
   d) xÂ² - 7x - 18 = 0
      (xÂ² - 7x + 49/4) - 18 - 49/4 = 0
      (x - 7/2)Â² - 121/4 = 0
      (x - 7/2)Â² = 121/4
      x - 7/2 = Â±11/2
      x = 7/2 Â± 11/2
      x = 9 or x = -2

8. a) 2xÂ² + 12x + 10 = 0
      2(xÂ² + 6x) + 10 = 0
      2(xÂ² + 6x + 9 - 9) + 10 = 0
      2(x + 3)Â² - 18 + 10 = 0
      2(x + 3)Â² - 8 = 0
      2(x + 3)Â² = 8
      (x + 3)Â² = 4
      x + 3 = Â±2
      x = -3 Â± 2
      x = -1 or x = -5
   
   b) 3xÂ² - 6x - 24 = 0
      3(xÂ² - 2x) - 24 = 0
      3(xÂ² - 2x + 1 - 1) - 24 = 0
      3(x - 1)Â² - 3 - 24 = 0
      3(x - 1)Â² - 27 = 0
      3(x - 1)Â² = 27
      (x - 1)Â² = 9
      x - 1 = Â±3
      x = 1 Â± 3
      x = 4 or x = -2
   
   c) -4xÂ² + 8x + 12 = 0
      -4(xÂ² - 2x) + 12 = 0
      -4(xÂ² - 2x + 1 - 1) + 12 = 0
      -4(x - 1)Â² + 4 + 12 = 0
      -4(x - 1)Â² + 16 = 0
      -4(x - 1)Â² = -16
      (x - 1)Â² = 4
      x - 1 = Â±2
      x = 1 Â± 2
      x = 3 or x = -1
   
   d) 5xÂ² + 20x + 15 = 0
      5(xÂ² + 4x) + 15 = 0
      5(xÂ² + 4x + 4 - 4) + 15 = 0
      5(x + 2)Â² - 20 + 15 = 0
      5(x + 2)Â² - 5 = 0
      5(x + 2)Â² = 5
      (x + 2)Â² = 1
      x + 2 = Â±1
      x = -2 Â± 1
      x = -1 or x = -3

9. a) xÂ² + 4x = 12
      xÂ² + 4x + 4 = 12 + 4
      (x + 2)Â² = 16
      x + 2 = Â±4
      x = -2 Â± 4
      x = 2 or x = -6
   
   b) xÂ² - 6x = -5
      xÂ² - 6x + 9 = -5 + 9
      (x - 3)Â² = 4
      x - 3 = Â±2
      x = 3 Â± 2
      x = 5 or x = 1
   
   c) 2xÂ² + 8x = 16
      2(xÂ² + 4x) = 16
      2(xÂ² + 4x + 4 - 4) = 16
      2(x + 2)Â² - 8 = 16
      2(x + 2)Â² = 24
      (x + 2)Â² = 12
      x + 2 = Â±2âˆš3
      x = -2 Â± 2âˆš3
      x â‰ˆ 1.46 or x â‰ˆ -5.46
   
   d) 3xÂ² - 12x = -9
      3(xÂ² - 4x) = -9
      3(xÂ² - 4x + 4 - 4) = -9
      3(x - 2)Â² - 12 = -9
      3(x - 2)Â² = 3
      (x - 2)Â² = 1
      x - 2 = Â±1
      x = 2 Â± 1
      x = 3 or x = 1

### Part D: Applications

10. Let w be the width of the garden and w + 3 be the length.
    Area = w(w + 3) = 70
    wÂ² + 3w = 70
    wÂ² + 3w - 70 = 0
    
    Complete the square:
    wÂ² + 3w + 9/4 - 9/4 - 70 = 0
    (w + 3/2)Â² - 9/4 - 70 = 0
    (w + 3/2)Â² = 9/4 + 70 = 9/4 + 280/4 = 289/4
    w + 3/2 = Â±17/2
    
    Since width must be positive, w = -3/2 + 17/2 = 7
    
    The dimensions of the garden are 7 meters by 10 meters.

11. a) h(t) = -4.9tÂ² + 20t + 2
       = -4.9(tÂ² - 20/-4.9t) + 2
       = -4.9(tÂ² - 4.08t) + 2
       = -4.9(tÂ² - 4.08t + 4.16 - 4.16) + 2
       = -4.9(t - 2.04)Â² + 20.38 + 2
       = -4.9(t - 2.04)Â² + 22.38
       Vertex form: h(t) = -4.9(t - 2.04)Â² + 22.38
    
    b) The maximum height is 22.38 meters.
    
    c) The ball reaches its maximum height at t = 2.04 seconds.
    
    d) The ball hits the ground when h(t) = 0:
       -4.9(t - 2.04)Â² + 22.38 = 0
       -4.9(t - 2.04)Â² = -22.38
       (t - 2.04)Â² = 22.38/4.9 â‰ˆ 4.57
       t - 2.04 = Â±âˆš4.57 â‰ˆ Â±2.14
       t = 2.04 Â± 2.14
       t = 4.18 or t = -0.1
       
       Since negative time doesn't make sense in this context, the ball hits the ground at approximately 4.18 seconds.

12. a) P(x) = -0.5xÂ² + 100x - 1000
       = -0.5(xÂ² - 200x) - 1000
       = -0.5(xÂ² - 200x + 10000 - 10000) - 1000
       = -0.5(x - 100)Â² + 5000 - 1000
       = -0.5(x - 100)Â² + 4000
       Vertex form: P(x) = -0.5(x - 100)Â² + 4000
    
    b) The profit is maximized when x = 100 items.
    
    c) The maximum profit is P(100) = 4000 dollars.
    
    d) To find the break-even points, set P(x) = 0:
       -0.5(x - 100)Â² + 4000 = 0
       -0.5(x - 100)Â² = -4000
       (x - 100)Â² = 8000
       x - 100 = Â±âˆš8000 â‰ˆ Â±89.44
       x = 100 Â± 89.44
       x â‰ˆ 189.44 or x â‰ˆ 10.56
       
       The break-even points are approximately 11 items and 189 items.

### Part E: Challenge Problems

13. f(x) = 2xÂ² - 8x + 13
    = 2(xÂ² - 4x) + 13
    = 2(xÂ² - 4x + 4 - 4) + 13
    = 2(x - 2)Â² - 8 + 13
    = 2(x - 2)Â² + 5
    
    The minimum value of f(x) is 5, which occurs at x = 2.

14. f(x) = axÂ² + bx + c (where a â‰  0)
    = a(xÂ² + b/aÂ·x) + c
    = a(xÂ² + b/aÂ·x + bÂ²/4aÂ² - bÂ²/4aÂ²) + c
    = a(x + b/2a)Â² - bÂ²/4a + c
    
    The vertex form is f(x) = a(x + b/2a)Â² + (c - bÂ²/4a)
    
    The x-coordinate of the vertex is -b/2a.

15. For a quadratic function with vertex at (3, -4) and passing through (5, 0):
    f(x) = a(x - 3)Â² - 4
    
    Since the function passes through (5, 0):
    0 = a(5 - 3)Â² - 4
    0 = 4a - 4
    4a = 4
    a = 1
    
    Therefore, f(x) = (x - 3)Â² - 4
